rustfrontend/RustIRsem.v
@@ -87,14 +87,14 @@ Variable ge: genv.
 Inductive step_drop : state -> trace -> state -> Prop :=
 | step_dropstate_init: forall id b ofs fid fty membs k m,
     step_drop (Dropstate id (Vptr b ofs) None ((Member_plain fid fty) :: membs) k m) E0 (Dropstate id (Vptr b ofs) (type_to_drop_member_state ge fid fty) membs k m)
-| step_dropstate_struct: forall id1 id2 co1 co2 b1 ofs1 cb cofs tys m k membs fid fty fofs bf orgs
+| step_dropstate_struct: forall id1 id2 co1 co2 b1 ofs1 cb cofs tys m k membs fid fty fofs  orgs
     (* step to another struct drop glue *)
     (CO1: ge.(genv_cenv) ! id1 = Some co1)
     (* evaluate the value of the argument for the drop glue of id2 *)
     (FOFS: match co1.(co_sv) with
            | Struct => field_offset ge fid co1.(co_members)
            | TaggedUnion => variant_field_offset ge fid co1.(co_members)
-           end = OK (fofs, bf))
+           end = OK fofs)
     (* (cb, cofs is the address of composite id2) *)
     (DEREF: deref_loc_rec m b1 (Ptrofs.add ofs1 (Ptrofs.repr fofs)) tys (Vptr cb cofs))
     (CO2: ge.(genv_cenv) ! id2 = Some co2)
@@ -102,14 +102,14 @@ Inductive step_drop : state -> trace -> state -> Prop :=
     step_drop
       (Dropstate id1 (Vptr b1 ofs1) (Some (drop_member_comp fid fty (Tstruct orgs id2) tys)) membs k m) E0
       (Dropstate id2 (Vptr cb cofs) None co2.(co_members) (Kdropcall id1 (Vptr b1 ofs1) (Some (drop_member_box fid fty tys)) membs k) m)
-| step_dropstate_enum: forall id1 id2 co1 co2 b1 ofs1 cb cofs tys m k membs fid1 fty1 fid2 fty2 fofs bf tag orgs
+| step_dropstate_enum: forall id1 id2 co1 co2 b1 ofs1 cb cofs tys m k membs fid1 fty1 fid2 fty2 fofs tag orgs
     (* step to another enum drop glue: remember to evaluate the switch statements *)
     (CO1: ge.(genv_cenv) ! id1 = Some co1)
     (* evaluate the value of the argument for the drop glue of id2 *)
     (FOFS: match co1.(co_sv) with
            | Struct => field_offset ge fid1 co1.(co_members)
            | TaggedUnion => variant_field_offset ge fid1 co1.(co_members)
-           end = OK (fofs, bf))
+           end = OK fofs)
     (* (cb, cofs is the address of composite id2) *)
     (DEREF: deref_loc_rec m b1 (Ptrofs.add ofs1 (Ptrofs.repr fofs)) tys (Vptr cb cofs))
     (CO2: ge.(genv_cenv) ! id2 = Some co2)
@@ -122,13 +122,13 @@ Inductive step_drop : state -> trace -> state -> Prop :=
     step_drop
       (Dropstate id1 (Vptr b1 ofs1) (Some (drop_member_comp fid1 fty1 (Tvariant orgs id2) tys)) membs k m) E0
       (Dropstate id2 (Vptr cb cofs) (type_to_drop_member_state ge fid2 fty2) nil (Kdropcall id1 (Vptr b1 ofs1) (Some (drop_member_box fid1 fty1 tys)) membs k) m)
-| step_dropstate_box: forall b ofs id co fid fofs bf m m' tys k membs fty
+| step_dropstate_box: forall b ofs id co fid fofs m m' tys k membs fty
     (CO1: ge.(genv_cenv) ! id = Some co)
     (* evaluate the value of the argument of the drop glue for id2 *)
     (FOFS: match co.(co_sv) with
            | Struct => field_offset ge fid co.(co_members)
            | TaggedUnion => variant_field_offset ge fid co.(co_members)
-           end = OK (fofs, bf))
+           end = OK fofs)
     (DROPB: drop_box_rec ge b (Ptrofs.add ofs (Ptrofs.repr fofs)) m tys m'),
     step_drop
       (Dropstate id (Vptr b ofs) (Some (drop_member_box fid fty tys)) membs k m) E0
@@ -145,38 +145,38 @@ Inductive step_drop : state -> trace -> state -> Prop :=
 
 
 Inductive step_drop_mem_error : state -> Prop :=
-| step_dropstate_struct_error: forall id1 id2 co1 b1 ofs1 tys m k membs fid fty fofs bf orgs
+| step_dropstate_struct_error: forall id1 id2 co1 b1 ofs1 tys m k membs fid fty fofs orgs
     (* step to another struct drop glue *)
     (CO1: ge.(genv_cenv) ! id1 = Some co1)
     (* evaluate the value of the argument for the drop glue of id2 *)
     (FOFS: match co1.(co_sv) with
            | Struct => field_offset ge fid co1.(co_members)
            | TaggedUnion => variant_field_offset ge fid co1.(co_members)
-           end = OK (fofs, bf))
+           end = OK fofs)
     (* error in loading the address of the composite *)
     (DEREF: deref_loc_rec_mem_error m b1 (Ptrofs.add ofs1 (Ptrofs.repr fofs)) tys),
     step_drop_mem_error
       (Dropstate id1 (Vptr b1 ofs1) (Some (drop_member_comp fid fty (Tstruct orgs id2) tys)) membs k m)
-| step_dropstate_enum_error1: forall id1 id2 co1 b1 ofs1 tys m k membs fid1 fty1 fofs bf orgs
+| step_dropstate_enum_error1: forall id1 id2 co1 b1 ofs1 tys m k membs fid1 fty1 fofs orgs
     (* step to another enum drop glue: remember to evaluate the switch statements *)
     (CO1: ge.(genv_cenv) ! id1 = Some co1)
     (* evaluate the value of the argument for the drop glue of id2 *)
     (FOFS: match co1.(co_sv) with
            | Struct => field_offset ge fid1 co1.(co_members)
            | TaggedUnion => variant_field_offset ge fid1 co1.(co_members)
-           end = OK (fofs, bf))
+           end = OK fofs)
     (* error in loading the address of the composite *)
     (DEREF: deref_loc_rec_mem_error m b1 (Ptrofs.add ofs1 (Ptrofs.repr fofs)) tys),
     step_drop_mem_error
     (Dropstate id1 (Vptr b1 ofs1) (Some (drop_member_comp fid1 fty1 (Tvariant orgs id2) tys)) membs k m)
-| step_dropstate_enum_error2: forall id1 id2 co1 co2 b1 ofs1 cb cofs tys m k membs fid1 fty1 fofs bf orgs
+| step_dropstate_enum_error2: forall id1 id2 co1 co2 b1 ofs1 cb cofs tys m k membs fid1 fty1 fofs orgs
     (* step to another enum drop glue: remember to evaluate the switch statements *)
     (CO1: ge.(genv_cenv) ! id1 = Some co1)
     (* evaluate the value of the argument for the drop glue of id2 *)
     (FOFS: match co1.(co_sv) with
            | Struct => field_offset ge fid1 co1.(co_members)
            | TaggedUnion => variant_field_offset ge fid1 co1.(co_members)
-           end = OK (fofs, bf))
+           end = OK fofs)
     (* (cb, cofs is the address of composite id2) *)
     (DEREF: deref_loc_rec m b1 (Ptrofs.add ofs1 (Ptrofs.repr fofs)) tys (Vptr cb cofs))
     (CO2: ge.(genv_cenv) ! id2 = Some co2)
@@ -185,13 +185,13 @@ Inductive step_drop_mem_error : state -> Prop :=
     (TAG: ~ Mem.valid_access m Mint32 cb (Ptrofs.unsigned cofs) Readable),
     step_drop_mem_error
       (Dropstate id1 (Vptr b1 ofs1) (Some (drop_member_comp fid1 fty1 (Tvariant orgs id2) tys)) membs k m)      
-| step_dropstate_box_error: forall b ofs id co fid fofs bf m tys k membs fty
+| step_dropstate_box_error: forall b ofs id co fid fofs m tys k membs fty
     (CO1: ge.(genv_cenv) ! id = Some co)
     (* evaluate the value of the argument of the drop glue for id2 *)
     (FOFS: match co.(co_sv) with
            | Struct => field_offset ge fid co.(co_members)
            | TaggedUnion => variant_field_offset ge fid co.(co_members)
-           end = OK (fofs, bf))
+           end = OK fofs)
     (* error in dropping the box chain *)
     (DROPB: drop_box_rec_mem_error ge b (Ptrofs.add ofs (Ptrofs.repr fofs)) m tys),
     step_drop_mem_error
